



I took all the parameters same as task 1
Because I designed my bike same as pendulum.

The equation describing the x-y coordinates of the pendulum position regarding its base are:-

$$x_p = -2l \sin \theta \quad \text{--- (i)}$$

$$y_p = 2l \cos \theta \quad \text{--- (ii)}$$

To find velocity components, taking the derivative

$$\dot{x}_p = -2l \dot{\theta} \cos \theta \quad \text{--- (3)}$$

$$\dot{y}_p = -2l \dot{\theta} \sin \theta \quad \text{--- (4)}$$

The speed of the arm along x-coordinate

$$V_{arm} = -R_p \dot{\alpha} \quad \text{--- (5)}$$

using (3) to (5), the velocity components of pendulum along the x and y direction

$$V_x = -R_p \dot{\alpha} - 2l \dot{\theta} \cos \theta \quad \text{--- (6)}$$

$$V_y = -2l \dot{\theta} \sin \theta \quad \text{--- (7)}$$

Now we know

$$L = E_{K.E.} - E_{P.E.}$$

$$E_{P.E.} = 2g m_p l \cos \theta \dots (8)$$

The total kinetic energy of the system. is equal to sum of kinetic energies of its moving parts as:-

$$\begin{aligned} E_{KE} &= K.E._{arm} + K.E._{pen} + K.E._{v_x} + K.E._{v_y} \\ &= \frac{1}{2} \times I_{arm} \times \dot{\alpha}^2 + \frac{1}{2} \times I_{pen} \times \dot{\theta}^2 + \frac{1}{2} m_p (2l)^2 \dot{\theta}^2 \sin^2 \theta \\ &\quad + \frac{1}{2} \times m_p \times (R_p)^2 \times \dot{\alpha}^2 \end{aligned}$$

$$\therefore K.E._{v_x} = \frac{1}{2} m_p v_x^2 \quad \therefore K.E._{v_y} = \frac{1}{2} m_p v_y^2$$

$$\text{Now } L = KE - PE$$

$$\begin{aligned} L &= \frac{1}{2} I_{arm} \dot{\alpha}^2 + \frac{1}{2} I_{pen} \dot{\theta}^2 + \frac{1}{2} m_p (2l)^2 \dot{\theta}^2 \sin^2 \theta + \\ &\quad \frac{1}{2} m_p (R_p)^2 \dot{\alpha}^2 + \frac{1}{2} m_p (2l)^2 \dot{\theta}^2 \cos^2 \theta \\ &\quad + m_p \dot{\alpha} (2l) (R_p) \dot{\theta} \cos \theta - 2g m_p l \cos \theta \end{aligned}$$

$$\begin{aligned} L &= \frac{1}{2} I_{arm} \dot{\alpha}^2 + \frac{1}{2} I_{pen} \dot{\theta}^2 + 2m_p l^2 \dot{\theta}^2 \sin^2 \theta + \\ &\quad \frac{1}{2} m_p R_p^2 \dot{\alpha}^2 + 2m_p l^2 \dot{\theta}^2 \cos^2 \theta + 2m_p \dot{\alpha}^2 l R_p \dot{\theta} \cos \theta \\ &\quad - 2g m_p l \cos \theta \dots (9) \end{aligned}$$

$$\frac{d}{dt} \left(\frac{\delta L}{\delta \dot{\alpha}} \right) - \frac{\delta L}{\delta \alpha} = T \quad \dots \quad (10)$$

$$\frac{d}{dt} \left(\frac{\delta L}{\delta \dot{\theta}} \right) - \frac{\delta L}{\delta \theta} = 0 \quad \dots \quad (11)$$

$$L = \frac{1}{2} I_{\text{arm}} \dot{\alpha}^2 + \frac{1}{2} I_{\text{pen}} \dot{\theta}^2 + 2Mpl^2 \dot{\theta}^2 \sin^2 \theta + \frac{1}{2} M_p R_p^2 \dot{\alpha}^2 + 2Mpl^2 \ddot{\theta}^2 \cos^2 \theta + 2Mpl \dot{\alpha} \perp R_p \dot{\theta} \cos \theta - 2gMpl \cos \theta \quad \dots \quad (12)$$

Substituting L in equation (10)

$$\left(\frac{\delta L}{\delta \alpha} \right) = 0 \quad \dots \quad (13)$$

$$\left(\frac{\delta L}{\delta \dot{\alpha}} \right) = I_{\text{arm}} \dot{\alpha} + M_p R_p^2 \dot{\alpha} + 2Mpl R_p \dot{\theta} \cos \theta \quad \dots \quad (14)$$

$$\frac{d}{dt} \left(\frac{\delta L}{\delta \dot{\alpha}} \right) = I_{\text{arm}} \ddot{\alpha} + M_p R_p^2 \ddot{\alpha} + 2Mpl R_p \ddot{\theta} \cos \theta - 2Mpl R_p \dot{\theta}^2 \sin \theta \quad \dots \quad (15)$$

From (10), (13), (15) equations

$$I_{\text{arm}} \ddot{\alpha} + M_p R_p^2 \ddot{\alpha} + 2Mpl R_p \ddot{\theta} \cos \theta - 2Mpl R_p \dot{\theta}^2 \sin \theta = T$$

$$I_{\text{arm}} \ddot{\alpha} + M_p R_p^2 \ddot{\alpha} + 2Mpl R_p \ddot{\theta} \cos \theta - 2Mpl R_p \dot{\theta}^2 \sin \theta = T$$

$$\left(\frac{\delta L}{\delta \dot{\theta}}\right) = -2Mpl\dot{\alpha}R_p\dot{\theta}\sin\theta + 2gMpl\sin\theta \dots (16)$$

$$\left(\frac{\delta L}{\delta \dot{\theta}}\right) = I_{-pen}\dot{\theta} + 4Mpl^2\dot{\theta}\sin^2\theta + 4Mpl^2\dot{\theta}\cos^2\theta + 2Mpl\dot{\alpha}R_p\cos\theta$$

$$\frac{d}{dt}\left(\frac{\delta L}{\delta \dot{\theta}}\right) = I_{-pen}\ddot{\theta} + 4Mpl^2\ddot{\theta} + 2MplR_p\ddot{\alpha}\cos\theta - \dot{\alpha}\dot{\theta}\sin\theta \dots (17)$$

From (11), (16), (17) equations

$$I_{-pen}\ddot{\theta} + 4Mpl^2\ddot{\theta} + 2MplR_p\ddot{\alpha}\cos\theta - \dot{\alpha}\dot{\theta}\sin\theta + 2Mpl\dot{\alpha}R_p\dot{\theta}\sin\theta - 2gMpl\sin\theta = 0$$

Now we have two equations:-

$$I_{-arm}\ddot{\alpha} + M_pR_p^2\ddot{\alpha} + 2MplR_p\ddot{\theta}\cos\theta - 2MplR_p\dot{\theta}^2\sin\theta = T$$

$$I_{-pen}\ddot{\theta} + 4Mpl^2\ddot{\theta} + 2MplR_p\ddot{\alpha}\cos\theta - \dot{\alpha}\dot{\theta}\sin\theta + 2Mpl\dot{\alpha}R_p\dot{\theta}\sin\theta - 2gMpl\sin\theta = 0$$

Using these two equation I got $\ddot{\alpha}$ and $\ddot{\theta}$ which is used in octave I will provide in pdf also.

$$\ddot{\alpha} = \frac{-T \cdot K_1 \cos \theta - K_1^2 \dot{\theta}^2 \sin \theta \cos \theta + 2K_1 K_6 \dot{\alpha} \dot{\theta} \sin \theta - K_5 K_6 \sin \theta - \dot{\alpha} \dot{\theta} K_6 \sin \theta}{-K_1^2 \cos^2 \theta - K_6 K_7}$$

$$\ddot{\theta} = \frac{\cos \theta \sin \theta [(K_1 \dot{\alpha} \dot{\theta} - 2K_1^2 \dot{\alpha} \dot{\theta} + K_1 K_5)] - K_7 T - K_1 K_7 \dot{\theta}^2 \sin \theta}{K_1^2 \cos^2 \theta - K_7 K_6}$$

Where

$$K_1 = 2 M_p l R_p$$

$$K_2 = 2 M_p l$$

$$K_3 = M_p R_p l^2$$

$$K_4 = M_p l^2$$

$$K_5 = 2 g M_p l$$

$$K_6 = I_{\text{arm}} + K_3$$

$$K_7 = I_{\text{pen}} + 4 K_4$$